messageInvariantPrototypes/toyLeaderElection/readme.md
@@ -1,0 +1,4 @@
+# Toy Leader Election
+
+In this system, because host states are already monotonic, there is no need for monotonic transformations.
+This is crazy.
